theories/L6_PCPS/cps_util.v
@@ -3,8 +3,8 @@
  *)
 
 From compcert.lib Require Import Coqlib.
-From CertiCoq.L6 Require Import cps ctx Ensembles_util List_util
-                                functions tactics map_util.
+Require Import L6.tactics.
+From CertiCoq.L6 Require Import cps ctx Ensembles_util List_util functions map_util.
 From Coq Require Import Arith.Arith NArith.BinNat Strings.String Lists.List
      omega.Omega Sets.Ensembles Relations.Relation_Operators Classes.Morphisms.
 From Template Require Import BasicAst. (* For identifier names *)
