theories/L6_PCPS/identifiers.v
@@ -6,7 +6,8 @@ From Coq Require Import Lists.List Lists.SetoidList NArith.BinNat PArith.BinPos
      MSets.MSetRBT Sets.Ensembles Omega Sorting.Permutation Logic.Decidable.
 
 From compcert.lib Require Import Coqlib.
-From CertiCoq.L6 Require Import cps cps_util ctx set_util Ensembles_util List_util tactics.
+Require Import L6.tactics.
+From CertiCoq.L6 Require Import cps cps_util ctx set_util Ensembles_util List_util.
 
 Import ListNotations.
 
